@prefix : <https://saref.etsi.org/saref4ehaw/> .
@prefix owl: <http://www.w3.org/2002/07/owl#> .
@prefix rdf: <http://www.w3.org/1999/02/22-rdf-syntax-ns#> .
@prefix xml: <http://www.w3.org/XML/1998/namespace> .
@prefix xsd: <http://www.w3.org/2001/XMLSchema#> .
@prefix foaf: <http://xmlns.com/foaf/0.1/> .
@prefix rdfs: <http://www.w3.org/2000/01/rdf-schema#> .
@prefix vann: <http://purl.org/vocab/vann/> .
@prefix voaf: <http://purl.org/vocommons/voaf#> .
@prefix saref: <https://saref.etsi.org/core/> .
@prefix s4ehaw: <https://saref.etsi.org/saref4ehaw/> .
@prefix s4envi: <https://saref.etsi.org/saref4envi/> .
@prefix dcterms: <http://purl.org/dc/terms/> .
@prefix ssn-system: <http://www.w3.org/ns/ssn/systems/> .
@base <https://saref.etsi.org/saref4ehaw/> .

<https://saref.etsi.org/saref4ehaw/> rdf:type owl:Ontology ;
                                      owl:versionIRI <https://saref.etsi.org/saref4ehaw/v1.1.1/> ;
                                      owl:imports <https://saref.etsi.org/core/v3.1.1/> ;
                                      dcterms:contributor <http://www.maxime-lefrancois.info/> ,
                                                          <https://pdi.fbk.eu/people/profile/dragoni> ,
                                                          <https://research.utwente.nl/en/persons/jo%C3%A3o-luiz-moreira> ,
                                                          <https://www.linkedin.com/in/lina-nachabe-2b292457/> ;
                                      dcterms:creator <http://www-public.imtbs-tsp.eu/~girodgen/> ;
                                      dcterms:description """The objective of SAREF4EHAW is to extend SAREF ontology for the eHealth/Ageing-well (EHAW) vertical. Clause 4.1 of the present document shortly introduces a high level view of the envisioned SAREF4EHAW semantic model and modular ontology, with the retained concepts (i.e. classes) and their relations. 
SAREF4EHAW extension has been specified and formalised by investigating EHAW domain related resources, as reported in ETSI TR 103 509, such as: potential stakeholders, standardization initiatives, alliances/associations, European projects, EC directives, existing ontologies, and data repositories. Therefore, SAREF4EHAW modular ontology shall both:
 - Allow the implementation of a limited set of typical EHAW related use cases already identified in ETSI TR 103 509, i.e.
 - Use case 1 “elderly at home monitoring and support”,
 - Use case 2 “monitoring and support of healthy lifestyles for citizens”,
 - Use case 3 “Early Warning System (EWS) and Cardiovascular Accidents detection”.
 - Fulfil the eHealth Ageing Well related requirements provided in ETSI TR 103 509, mainly the ontological ones that were mostly taken as input for the ontology specification.

SAREF4EHAW mainly reuses the following existing ontologies: SAREF, ETSI SmartBAN reference model, SAREF 4 Environment extension and W3C SSN System module. The following figure presents the high level view of SAREF4EHAW ontology.
![SAREF4SYST overview](diagrams/SAREF4EHAW_Model.jpg)
For semantic interoperability handling purposes, an ontology based solution, combined with sensing-as-a-service and WoT strategies, is retained for SAREF4EHAW. Therefore, an upper level ontology, at service level, shall also behas been fully modelled (Service class and sub-classes depicted in the previous figure).
For embedded semantic analytics purposes, SAREF4EHAW shall behas been designed using the modularity principle (see ETSI TR 103 509) and can thus be mainly described by the following self-contained knowledge sub-ontologies (or modules): HealthActor, Ban, HealthDevice, Function (measured data related concepts included) and Service."""^^<https://www.iana.org/assignments/media-types/text/markdown> ;
                                      dcterms:issued "2020-02-01"^^xsd:date ;
                                      dcterms:license <https://forge.etsi.org/etsi-software-license> ;
                                      dcterms:modified "2020-05-01"^^xsd:date ;
                                      dcterms:publisher <https://www.etsi.org/> ;
                                      dcterms:source <https://saref.etsi.org/sources/saref4ehaw/> ;
                                      dcterms:title "SAREF4EHAW: an extension of SAREF for eHealth Ageing Well domain"@en ;
                                      vann:preferredNamespacePrefix "s4ehaw" ;
                                      vann:preferredNamespaceUri "https://saref.etsi.org/saref4ehaw/" ;
                                      rdfs:seeAlso <https://www.etsi.org/deliver/etsi_ts/103400_103499/10341008/01.01.01_60/ts_10341008v010101p.pdf> ;
                                      owl:versionInfo "v1.1.1" .

#################################################################
#    Annotation properties
#################################################################

###  http://purl.org/dc/terms/contributor
dcterms:contributor rdf:type owl:AnnotationProperty .


###  http://purl.org/dc/terms/creator
dcterms:creator rdf:type owl:AnnotationProperty .


###  http://purl.org/dc/terms/description
dcterms:description rdf:type owl:AnnotationProperty .


###  http://purl.org/dc/terms/issued
dcterms:issued rdf:type owl:AnnotationProperty .


###  http://purl.org/dc/terms/license
dcterms:license rdf:type owl:AnnotationProperty .


###  http://purl.org/dc/terms/modified
dcterms:modified rdf:type owl:AnnotationProperty .


###  http://purl.org/dc/terms/publisher
dcterms:publisher rdf:type owl:AnnotationProperty .


###  http://purl.org/dc/terms/source
dcterms:source rdf:type owl:AnnotationProperty .


###  http://purl.org/dc/terms/title
dcterms:title rdf:type owl:AnnotationProperty .


###  http://purl.org/vocab/vann/preferredNamespacePrefix
vann:preferredNamespacePrefix rdf:type owl:AnnotationProperty .


###  http://purl.org/vocab/vann/preferredNamespaceUri
vann:preferredNamespaceUri rdf:type owl:AnnotationProperty .


#################################################################
#    Datatypes
#################################################################

###  https://www.iana.org/assignments/media-types/text/markdown
<https://www.iana.org/assignments/media-types/text/markdown> rdf:type rdfs:Datatype .


#################################################################
#    Object Properties
#################################################################

###  https://saref.etsi.org/core/consistsOf
saref:consistsOf rdf:type owl:ObjectProperty ;
                 rdfs:comment "A relationship indicating a composite entity that consists of other entities (e.g., a temperature/humidity sensor that consists of a temperature sensor and a humidity sensor)"@en ;
                 rdfs:isDefinedBy saref: ;
                 rdfs:label "consists of"@en .


###  https://saref.etsi.org/saref4ehaw/contains
s4ehaw:contains rdf:type owl:ObjectProperty ;
                rdfs:domain s4ehaw:Ban ;
                rdfs:range s4ehaw:HealthDevice ;
                rdfs:comment "A Body Area Network or BAN contains one or multiple health devices"@en ;
                rdfs:label "contains"@en .


###  https://saref.etsi.org/saref4ehaw/followsUser
s4ehaw:followsUser rdf:type owl:ObjectProperty ;
                   rdfs:domain s4ehaw:Helper ;
                   rdfs:range s4ehaw:User ;
                   rdfs:comment "A helper may follow one or multiple users that can in particular be patients."@en ;
                   rdfs:label "follows user"@en .


###  https://saref.etsi.org/saref4ehaw/groundingProtocol
s4ehaw:groundingProtocol rdf:type owl:ObjectProperty ;
                         rdfs:domain s4ehaw:ServiceGrounding ;
                         rdfs:range s4ehaw:CommunicationProtocol ;
                         rdfs:comment "The grounding protocol is the protocol used to transmit the message by the service, e.g. BLE."@en ;
                         rdfs:label "grounding protocol"@en .


###  https://saref.etsi.org/saref4ehaw/hasActivity
s4ehaw:hasActivity rdf:type owl:ObjectProperty ;
                   rdfs:domain s4ehaw:HealthActor ;
                   rdfs:range s4ehaw:Activity ;
                   rdfs:comment "A health actor may have one or multiple activities."@en ;
                   rdfs:label "has activity"@en .


###  https://saref.etsi.org/saref4ehaw/hasAgeCategory
s4ehaw:hasAgeCategory rdf:type owl:ObjectProperty ;
                      rdfs:domain s4ehaw:HealthActor ;
                      rdfs:range s4ehaw:AgeCategory ;
                      rdfs:comment "The age group of a health actor, e.g. old or young."@en ;
                      rdfs:label "has age category"@en .


###  https://saref.etsi.org/saref4ehaw/hasBanApplicationDomain
s4ehaw:hasBanApplicationDomain rdf:type owl:ObjectProperty ;
                               rdfs:domain s4ehaw:Ban ;
                               rdfs:range s4ehaw:BanApplicationDomain ;
                               rdfs:comment "The BAN application domain - healthcare, telemedicine, assisted living, sport training, pervasive computing, safety and emergency... -."@en ;
                               rdfs:label "has BAN application domain"@en .


###  https://saref.etsi.org/saref4ehaw/hasBanCommunicationType
s4ehaw:hasBanCommunicationType rdf:type owl:ObjectProperty ;
                               rdfs:domain s4ehaw:Ban ;
                               rdfs:range s4ehaw:BanCommunicationType ;
                               rdfs:comment "A BAN has a BAN communication type that is the type of communication carried out between BAN devices and BAN Hub."@en ;
                               rdfs:label "has BAN communication type"@en .


###  https://saref.etsi.org/saref4ehaw/hasChronicDisease
s4ehaw:hasChronicDisease rdf:type owl:ObjectProperty ;
                         rdfs:domain s4ehaw:Patient ;
                         rdfs:range s4ehaw:ChronicDisease ;
                         rdfs:comment "A patient can suffer from one or more chronic disease like Diabetes, azma, etc."@en ;
                         rdfs:label "has chronic disease"@en .


###  https://saref.etsi.org/saref4ehaw/hasComputingPower
s4ehaw:hasComputingPower rdf:type owl:ObjectProperty ;
                         rdfs:domain s4ehaw:DeviceCharacteristic ;
                         rdfs:range s4ehaw:ComputingPower ;
                         rdfs:comment "A health device characteristic describing the processing power or capabilities of the device (e.g. processor ID and manufacturer, duty cycle, available flash/RM memory, maximum flash/RAM memory...)."@en ;
                         rdfs:label "has computing power"@en .


###  https://saref.etsi.org/saref4ehaw/hasContact
s4ehaw:hasContact rdf:type owl:ObjectProperty ;
                  rdfs:domain s4ehaw:Ban ;
                  rdfs:range s4ehaw:Contact ;
                  rdfs:comment "A BAN has one or multiple contacts (e.g. the patient or user that is monitored through this BAN, the caregiver that is using this BAN for monitoring purposes)."@en ;
                  rdfs:label "has contact"@en .


###  https://saref.etsi.org/saref4ehaw/hasData
s4ehaw:hasData rdf:type owl:ObjectProperty ;
               rdfs:domain saref:Function ;
               rdfs:range s4ehaw:Data ;
               rdfs:comment "A function has one or many data, for example a tracking function shall include latitude, longitude and speed data."@en ;
               rdfs:label "has data"@en .


###  https://saref.etsi.org/saref4ehaw/hasDataConstraint
s4ehaw:hasDataConstraint rdf:type owl:ObjectProperty ;
                         rdfs:domain s4ehaw:Data ;
                         rdfs:range s4ehaw:DataConstraint ;
                         rdfs:comment "Data has data constraints (validity, legal...)."@en ;
                         rdfs:label "has data constraint"@en .


###  https://saref.etsi.org/saref4ehaw/hasDeviceCharacteristic
s4ehaw:hasDeviceCharacteristic rdf:type owl:ObjectProperty ;
                               rdfs:domain s4ehaw:HealthDevice ;
                               rdfs:range s4ehaw:DeviceCharacteristic ;
                               rdfs:comment "A health device has device characteristic describing the physical characteristics of the health device, e.g. its dimensions."@en ;
                               rdfs:label "has device characteristic"@en .


###  https://saref.etsi.org/saref4ehaw/hasHabit
s4ehaw:hasHabit rdf:type owl:ObjectProperty ;
                rdfs:domain s4ehaw:User ;
                rdfs:range s4ehaw:Habit ;
                rdfs:comment "The habits of a user and a patient (as sub-class of user it also inherits habit), e.g. smoking or overeating."@en ;
                rdfs:label "has habit"@en .


###  https://saref.etsi.org/saref4ehaw/hasHub
s4ehaw:hasHub rdf:type owl:ObjectProperty ;
              rdfs:domain s4ehaw:Ban ;
              rdfs:range s4ehaw:BanHub ;
              rdfs:comment "A Body Area Network or BAN elects one hub that mainly plays the role of both a data concentrator and a network gateway."@en ;
              rdfs:label "has hub"@en .


###  https://saref.etsi.org/saref4ehaw/hasImpairment
s4ehaw:hasImpairment rdf:type owl:ObjectProperty ;
                     rdfs:domain s4ehaw:User ;
                     rdfs:range s4ehaw:Impairment ;
                     rdfs:comment "The impairment type of a user and a patient (as sub-class of user it also inherits impairment), e.g. aural, skeletal, ocular, mobility, intellectual..."@en ;
                     rdfs:label "has impairment"@en .


###  https://saref.etsi.org/saref4ehaw/hasInterface
s4ehaw:hasInterface rdf:type owl:ObjectProperty ;
                    rdfs:domain s4ehaw:HealthDevice ;
                    rdfs:range s4ehaw:Interface ;
                    rdfs:comment "A health device has one or multiple interfaces (Bluetooth, UWB, IEEE 802.15.6, serial interface...)."@en ;
                    rdfs:label "has interface"@en .


###  https://saref.etsi.org/saref4ehaw/hasLocation
s4ehaw:hasLocation rdf:type owl:ObjectProperty ;
                   rdfs:domain s4ehaw:HealthDevice ;
                   rdfs:range s4ehaw:Location ;
                   rdfs:comment "The location of an eHealth device, i.e. its position against the body (on body surface or in the body - implant -) and its physical location (i.e. its postal address and/or its current geolocation geolocation when available)."@en ;
                   rdfs:label "has location"@en .


###  https://saref.etsi.org/saref4ehaw/hasMeasurement
s4ehaw:hasMeasurement rdf:type owl:ObjectProperty ;
                      rdfs:domain s4ehaw:Data ;
                      rdfs:range saref:Measurement ;
                      rdfs:comment "Defines the relationship between data that has measurement."@en ;
                      rdfs:label "has measurement"@en .


###  https://saref.etsi.org/saref4ehaw/hasMode
s4ehaw:hasMode rdf:type owl:ObjectProperty ;
               rdfs:domain s4ehaw:DeviceCharacteristic ;
               rdfs:range s4ehaw:Mode ;
               rdfs:comment "Each device has modes of operations that model its dynamic characteristic varying during its lifetime, e.g. active, hold, beacon..."@en ;
               rdfs:label "has mode"@en .


###  https://saref.etsi.org/saref4ehaw/hasOperatingConstraint
s4ehaw:hasOperatingConstraint rdf:type owl:ObjectProperty ;
                              rdfs:domain s4ehaw:HealthDevice ;
                              rdfs:range s4ehaw:OperatingConstraint ;
                              rdfs:comment "The operating constraints of a health device, e.g. recommended humidity and temperature range..."@en ;
                              rdfs:label "has operating constraint"@en .


###  https://saref.etsi.org/saref4ehaw/hasParticipant
s4ehaw:hasParticipant rdf:type owl:ObjectProperty ;
                      rdfs:domain s4ehaw:MeasurementCollectionSession ;
                      rdfs:range s4ehaw:HealthActor ;
                      rdfs:comment "A measurement session has health actors as participants (caregiver controling the session, patient monitored during the session)."@en ;
                      rdfs:label "has participant"@en .


###  https://saref.etsi.org/saref4ehaw/hasPatient
s4ehaw:hasPatient rdf:type owl:ObjectProperty ;
                  rdfs:domain s4ehaw:Caregiver ;
                  rdfs:range s4ehaw:Patient ;
                  rdfs:comment "A caregiver may have one or multiple patients."@en ;
                  rdfs:label "has patient"@en .


###  https://saref.etsi.org/saref4ehaw/hasPhysicalLocation
s4ehaw:hasPhysicalLocation rdf:type owl:ObjectProperty ;
                           rdfs:domain s4ehaw:Patient ;
                           rdfs:range s4ehaw:PhysicalLocation ;
                           rdfs:comment "Defines the physical location of the patient, i.e. its postal address and/or its geolocation (when available)."@en ;
                           rdfs:label "has physical location"@en .


###  https://saref.etsi.org/saref4ehaw/hasPosture
s4ehaw:hasPosture rdf:type owl:ObjectProperty ;
                  rdfs:domain s4ehaw:User ;
                  rdfs:range s4ehaw:Posture ;
                  rdfs:comment "The posture of a user and a patient (as sub-class of user it also inherits habit), e.g. exercising, lying, running, sitting, walking..."@en ;
                  rdfs:label "has posture"@en .


###  https://saref.etsi.org/saref4ehaw/hasPowerSource
s4ehaw:hasPowerSource rdf:type owl:ObjectProperty ;
                      rdfs:domain s4ehaw:DeviceCharacteristic ;
                      rdfs:range s4ehaw:PowerSource ;
                      rdfs:comment "A health device characteristic is its  power sources, mainly describing energy source and battery related capabilities of the health device (number of power source, source type, rechargeable or not, available power level...)."@en ;
                      rdfs:label "has power source"@en .


###  https://saref.etsi.org/saref4ehaw/hasResponsibleParty
s4ehaw:hasResponsibleParty rdf:type owl:ObjectProperty ;
                           rdfs:domain s4ehaw:Ban ;
                           rdfs:range s4ehaw:ResponsibleParty ;
                           rdfs:comment "A BAN that has a responsible party which plays the role of the legal entity responsible for this BAN (e.g. to contact in case of problem). It should be an organization or a person."@en ;
                           rdfs:label "has responsible party"@en .


###  https://saref.etsi.org/saref4ehaw/hasTimeSeriesMesurement
s4ehaw:hasTimeSeriesMesurement rdf:type owl:ObjectProperty ;
                               rdfs:domain s4ehaw:Data ;
                               rdfs:range s4ehaw:TimeSeriesMeasurement ;
                               rdfs:comment "Data has time series measurements, a sequence taken at successive equally spaced points in time."@en ;
                               rdfs:label "has time series measurement"@en .


###  https://saref.etsi.org/saref4ehaw/inCurrentMode
s4ehaw:inCurrentMode rdf:type owl:ObjectProperty ;
                     rdfs:domain s4ehaw:HealthDevice ;
                     rdfs:range s4ehaw:Mode ;
                     rdfs:comment "Each eHealth device has modes of operations that model its dynamic characteristic varying during its lifetime, e.g. active, hold, beacon..."@en ;
                     rdfs:label "in current mode"@en .


###  https://saref.etsi.org/saref4ehaw/interfaceProtocol
s4ehaw:interfaceProtocol rdf:type owl:ObjectProperty ;
                         rdfs:domain s4ehaw:Interface ;
                         rdfs:range s4ehaw:CommunicationProtocol ;
                         rdfs:comment "The interface communication protocol can be e.g. BLE, serial, Ethernet..."@en ;
                         rdfs:label "interface protocol"@en .


###  https://saref.etsi.org/saref4ehaw/isAttachedTo
s4ehaw:isAttachedTo rdf:type owl:ObjectProperty ;
                    rdfs:domain s4ehaw:HealthDevice ;
                    rdfs:range s4ehaw:HealthActor ;
                    rdfs:comment "A health Device is attached to a health actor such as a patient, a user and or a caregiver."@en ;
                    rdfs:label "is attached to"@en .


###  https://saref.etsi.org/saref4ehaw/isDescribedBy
s4ehaw:isDescribedBy rdf:type owl:ObjectProperty ;
                     rdfs:domain saref:Service ;
                     rdfs:range s4ehaw:ServiceProcess ;
                     rdfs:comment "A service is described by a service process (how the service works)."@en ;
                     rdfs:label "is described by"@en .


###  https://saref.etsi.org/saref4ehaw/precision
s4ehaw:precision rdf:type owl:ObjectProperty ;
                 rdfs:domain s4ehaw:MeasurementFunction ;
                 rdfs:range ssn-system:Precision ;
                 rdfs:comment "Precision refers to the degree of reproducibility of a measured quantity (when the same quantity is measured several times how close are the measurements from each other)."@en ;
                 rdfs:label "precision"@en .


###  https://saref.etsi.org/saref4ehaw/presents
s4ehaw:presents rdf:type owl:ObjectProperty ;
                rdfs:domain saref:Service ;
                rdfs:range s4ehaw:ServiceProfile ;
                rdfs:comment "A service presents a service profile (what the service does)."@en ;
                rdfs:label "presents"@en .


###  https://saref.etsi.org/saref4ehaw/supports
s4ehaw:supports rdf:type owl:ObjectProperty ;
                rdfs:domain saref:Service ;
                rdfs:range s4ehaw:ServiceGrounding ;
                rdfs:comment "A service supports a service grounding (how to access the service)." ;
                rdfs:label "supports"@en .


###  https://saref.etsi.org/saref4ehaw/uom
s4ehaw:uom rdf:type owl:ObjectProperty ;
           rdfs:domain s4ehaw:MeasurementFunction ;
           rdfs:range saref:UnitOfMeasure ;
           rdfs:comment "Defines the unit of measure of a measurement function."@en ;
           rdfs:label "unit of measurement"@en .


###  https://saref.etsi.org/saref4ehaw/usesBan
s4ehaw:usesBan rdf:type owl:ObjectProperty ;
               rdfs:domain s4ehaw:HealthActor ;
               rdfs:range s4ehaw:Ban ;
               rdfs:comment "A health actor (e.g. a caregiver, a patient or a helper) uses a BAN for collecting, aggregating and relaying vital parameters."@en ;
               rdfs:label "uses ban"@en .


###  https://saref.etsi.org/saref4envi/hasFrequencyMeasurement
s4envi:hasFrequencyMeasurement rdf:type owl:ObjectProperty ;
                               rdfs:domain s4ehaw:MeasurementFunction ;
                               rdfs:range s4envi:FrequencyMeasurement ;
                               rdfs:comment "A measurement fucntion, in case of complex measurement like time series, has frequency measurement, i.e. the frequency in which it makes measurements."@en ;
                               rdfs:label "has frequency measurement"@en .


#################################################################
#    Data properties
#################################################################

###  https://saref.etsi.org/core/hasManufacturer
saref:hasManufacturer rdf:type owl:DatatypeProperty ;
                      rdfs:comment "A relationship identifying the manufacturer of an entity (e.g., device). The value is expected to be a string or a string with language tag."@en ;
                      rdfs:isDefinedBy saref: ;
                      rdfs:label "has manufacturer"@en .


###  https://saref.etsi.org/saref4ehaw/activityDuration
s4ehaw:activityDuration rdf:type owl:DatatypeProperty ;
                        rdfs:domain s4ehaw:Activity ;
                        rdfs:range xsd:float ;
                        rdfs:comment "The duration of an activity, in second."@en ;
                        rdfs:label "activity duration"@en .


###  https://saref.etsi.org/saref4ehaw/activityKind
s4ehaw:activityKind rdf:type owl:DatatypeProperty ;
                    rdfs:domain s4ehaw:Activity ;
                    rdfs:range xsd:string ;
                    rdfs:comment "The kind of atcivities that a patient or a user can have, i.e. e.g. sleeping in bed, sitting on a chair, using the shower, etc."@en ;
                    rdfs:label "activity kind"@en .


###  https://saref.etsi.org/saref4ehaw/availableFlash
s4ehaw:availableFlash rdf:type owl:DatatypeProperty ;
                      rdfs:domain s4ehaw:HealthDevice ;
                      rdfs:range xsd:long ;
                      rdfs:comment "The available flash memory (in byte) of a health device. It is a dynamic attribute."@en ;
                      rdfs:label "available flash"@en .


###  https://saref.etsi.org/saref4ehaw/availableRam
s4ehaw:availableRam rdf:type owl:DatatypeProperty ;
                    rdfs:domain s4ehaw:HealthDevice ;
                    rdfs:range xsd:long ;
                    rdfs:comment "Indicates the available volatile memory space (in byte) of a health device. It is a dynamic attribute."@en ;
                    rdfs:label "available ram"@en .


###  https://saref.etsi.org/saref4ehaw/banDensity
s4ehaw:banDensity rdf:type owl:DatatypeProperty ;
                  rdfs:domain s4ehaw:Ban ;
                  rdfs:range xsd:long ;
                  rdfs:comment "The BAN density, i.e. its number of node."@en ;
                  rdfs:label "BAN density"@en .


###  https://saref.etsi.org/saref4ehaw/banGeolocation
s4ehaw:banGeolocation rdf:type owl:DatatypeProperty ;
                      rdfs:domain s4ehaw:Ban ;
                      rdfs:range xsd:string ;
                      rdfs:comment "The geolocation of the BAN, when available and needed, shall be given relatively to the current location - geolocation as standardized ISO 6709, e.g. +40.75-074.00/  - of the patient wearing the BAN."@en ;
                      rdfs:label "BAN geolocation"@en .


###  https://saref.etsi.org/saref4ehaw/banTopology
s4ehaw:banTopology rdf:type owl:DatatypeProperty ;
                   rdfs:domain s4ehaw:Ban ;
                   rdfs:range [ rdf:type rdfs:Datatype ;
                                owl:oneOf [ rdf:type rdf:List ;
                                            rdf:first "Adhoc" ;
                                            rdf:rest [ rdf:type rdf:List ;
                                                       rdf:first "Mesh" ;
                                                       rdf:rest [ rdf:type rdf:List ;
                                                                  rdf:first "Star" ;
                                                                  rdf:rest rdf:nil
                                                                ]
                                                     ]
                                          ]
                              ] ;
                   rdfs:comment "The BAN physical topology type, i.e Adhoc or Star or Mesh or Others."@ne ;
                   rdfs:label "BAN topology"@en .


###  https://saref.etsi.org/saref4ehaw/dataSize
s4ehaw:dataSize rdf:type owl:DatatypeProperty ;
                rdfs:domain s4ehaw:Data ;
                rdfs:range xsd:positiveInteger ;
                rdfs:comment "The data size represents the size of the data in bytes"@en ;
                rdfs:label "data size"@en .


###  https://saref.etsi.org/saref4ehaw/deviceCharacteristicName
s4ehaw:deviceCharacteristicName rdf:type owl:DatatypeProperty ;
                                rdfs:domain s4ehaw:DeviceCharacteristic ;
                                rdfs:range xsd:string ;
                                rdfs:comment "The commercial name of a device."@en ;
                                rdfs:label "device characteristic name"@en .


###  https://saref.etsi.org/saref4ehaw/dimension
s4ehaw:dimension rdf:type owl:DatatypeProperty ;
                 rdfs:domain s4ehaw:DeviceCharacteristic ;
                 rdfs:range xsd:string ;
                 rdfs:comment "The dimension of the device i.e. height*weight*length string."@en ;
                 rdfs:label "dimension"@en .


###  https://saref.etsi.org/saref4ehaw/dob
s4ehaw:dob rdf:type owl:DatatypeProperty ;
           rdfs:domain s4ehaw:HealthActor ;
           rdfs:range xsd:dateTime ;
           rdfs:comment "The date of birth of a health actor."@en ;
           rdfs:label "date of birth"@en .


###  https://saref.etsi.org/saref4ehaw/dutyCycle
s4ehaw:dutyCycle rdf:type owl:DatatypeProperty ;
                 rdfs:domain s4ehaw:ComputingPower ;
                 rdfs:range xsd:int ;
                 rdfs:comment "The duty cycle for each health device embedded processor, in percent."@en ;
                 rdfs:label "duty cycle"@en .


###  https://saref.etsi.org/saref4ehaw/faultTolerence
s4ehaw:faultTolerence rdf:type owl:DatatypeProperty ;
                      rdfs:domain s4ehaw:MeasurementFunction ;
                      rdfs:range xsd:double ;
                      rdfs:comment "Defines the error rate tolerated for a measurement function."@en ;
                      rdfs:label "fault tolerence"@en .


###  https://saref.etsi.org/saref4ehaw/firstName
s4ehaw:firstName rdf:type owl:DatatypeProperty ;
                 rdfs:domain s4ehaw:HealthActor ;
                 rdfs:range xsd:string ;
                 rdfs:comment "The first name of a health actor."@en ;
                 rdfs:label "first name"@en .


###  https://saref.etsi.org/saref4ehaw/format
s4ehaw:format rdf:type owl:DatatypeProperty ;
              rdfs:domain s4ehaw:Data ;
              rdfs:range xsd:anyURI ;
              rdfs:comment "The format is a URI for a standard format like e.g. integer."@en ;
              rdfs:label "format"@en .


###  https://saref.etsi.org/saref4ehaw/frequency
s4ehaw:frequency rdf:type owl:DatatypeProperty ;
                 rdfs:domain s4ehaw:ComputingPower ;
                 rdfs:range xsd:float ;
                 rdfs:comment "The frequency is the number of instructions an embedded processor - within a health device - can perform per second (MIPS)."@en ;
                 rdfs:label "frequency"@en .


###  https://saref.etsi.org/saref4ehaw/geolocation
s4ehaw:geolocation rdf:type owl:DatatypeProperty ;
                   rdfs:domain s4ehaw:PhysicalLocation ;
                   rdfs:range xsd:string ;
                   rdfs:comment "The geolocation, when available, shall be given relatively to the current location - geolocation as standardized ISO 6709, e.g. +40.75-074.00/ -."@en ;
                   rdfs:label "geolocation"@en .


###  https://saref.etsi.org/saref4ehaw/hasCalculationMethod
s4ehaw:hasCalculationMethod rdf:type owl:DatatypeProperty ;
                            rdfs:domain s4ehaw:ServiceProcess ;
                            rdfs:range xsd:string ;
                            rdfs:comment "The service process has a calculation method to get the output or result, e.g. the calculation formula to determine the posture of a patient."@en ;
                            rdfs:label "has calculation method"@en .


###  https://saref.etsi.org/saref4ehaw/hasEffect
s4ehaw:hasEffect rdf:type owl:DatatypeProperty ;
                 rdfs:domain s4ehaw:ServiceProcess ;
                 rdfs:range xsd:string ;
                 rdfs:comment "The effect of a service can be an alert, nothing, an activation of another process..."@en ;
                 rdfs:label "has effect"@en .


###  https://saref.etsi.org/saref4ehaw/hasGender
s4ehaw:hasGender rdf:type owl:DatatypeProperty ;
                 rdfs:domain s4ehaw:HealthActor ;
                 rdfs:range [ rdf:type rdfs:Datatype ;
                              owl:oneOf [ rdf:type rdf:List ;
                                          rdf:first "female" ;
                                          rdf:rest [ rdf:type rdf:List ;
                                                     rdf:first "male" ;
                                                     rdf:rest [ rdf:type rdf:List ;
                                                                rdf:first "undetermined" ;
                                                                rdf:rest rdf:nil
                                                              ]
                                                   ]
                                        ]
                            ] ;
                 rdfs:comment "The gender of a health actor."@en ;
                 rdfs:label "has gender"@en .


###  https://saref.etsi.org/saref4ehaw/hasInput
s4ehaw:hasInput rdf:type owl:DatatypeProperty ;
                rdfs:domain s4ehaw:ServiceProcess ;
                rdfs:range xsd:string ;
                rdfs:comment "The service process has data input like e.g. the patient ID, the timestamp, the read value from a sensor..."@en ;
                rdfs:label "has input"@en .


###  https://saref.etsi.org/saref4ehaw/hasMbox
s4ehaw:hasMbox rdf:type owl:DatatypeProperty ;
               rdfs:domain s4ehaw:HealthActor ;
               rdfs:range xsd:anyURI ;
               rdfs:comment "An email address (or mail box) of an health actor: a URI with the 'mailto' scheme as defined by RFC 6068."@en ;
               rdfs:label "has mbox"@en .


###  https://saref.etsi.org/saref4ehaw/hasOutput
s4ehaw:hasOutput rdf:type owl:DatatypeProperty ;
                 rdfs:domain s4ehaw:ServiceProcess ;
                 rdfs:range xsd:string ;
                 rdfs:comment "The output is e.g. the calculated value returned by the process, e.g the posture of a patient."@en ;
                 rdfs:label "has output"@en .


###  https://saref.etsi.org/saref4ehaw/hasPrecondition
s4ehaw:hasPrecondition rdf:type owl:DatatypeProperty ;
                       rdfs:domain s4ehaw:ServiceProcess ;
                       rdfs:range xsd:string ;
                       rdfs:comment "The conditions that are imposed over the inputs of the process and the process must hold to be successufully invoked."@en ;
                       rdfs:label "has precondition"@en .


###  https://saref.etsi.org/saref4ehaw/hasResult
s4ehaw:hasResult rdf:type owl:DatatypeProperty ;
                 rdfs:domain s4ehaw:ServiceProcess ;
                 rdfs:range xsd:string ;
                 rdfs:comment "The process can have many results for the same output. Those results may include a message that should be displayed, an alert..."@en ;
                 rdfs:label "has result"@en .


###  https://saref.etsi.org/saref4ehaw/hasValues
s4ehaw:hasValues rdf:type owl:DatatypeProperty ;
                 rdfs:domain s4ehaw:TimeSeriesMeasurement ;
                 rdfs:range xsd:decimal ;
                 rdfs:comment "A relationship defining the set of values (an ordered array of numbers) of a certain property, e.g., heart rate. Attention: to assure ordering in the serialization format, it is necessary to use either rdf:Seq (RDF/XML) or @list (JSON-LD)."@en ;
                 rdfs:label "has values"@en .


###  https://saref.etsi.org/saref4ehaw/interfaceAddress
s4ehaw:interfaceAddress rdf:type owl:DatatypeProperty ;
                        rdfs:domain s4ehaw:Interface ;
                        rdfs:range xsd:string ;
                        rdfs:comment "The interface address. The interface may have many addresses like MAC address, IP address or others."@en ;
                        rdfs:label "interface address"@en .


###  https://saref.etsi.org/saref4ehaw/interfaceDescription
s4ehaw:interfaceDescription rdf:type owl:DatatypeProperty ;
                            rdfs:domain s4ehaw:Interface ;
                            rdfs:range xsd:string ;
                            rdfs:comment "The interface type description."@en ;
                            rdfs:label "interface description"@en .


###  https://saref.etsi.org/saref4ehaw/isDerivedData
s4ehaw:isDerivedData rdf:type owl:DatatypeProperty ;
                     rdfs:domain s4ehaw:Data ;
                     rdfs:range xsd:boolean ;
                     rdfs:comment "Is derived data is a Boolean property to indicate if the data is a row data or a calculated/derived data from other one."@en ;
                     rdfs:label "is derived data"@en .


###  https://saref.etsi.org/saref4ehaw/isGateway
s4ehaw:isGateway rdf:type owl:DatatypeProperty ;
                 rdfs:domain s4ehaw:Interface ;
                 rdfs:range xsd:boolean ;
                 rdfs:comment "This boolean variable indicates if the interface is a gateway or not."@en ;
                 rdfs:label "is gateway"@en .


###  https://saref.etsi.org/saref4ehaw/lastName
s4ehaw:lastName rdf:type owl:DatatypeProperty ;
                rdfs:domain s4ehaw:HealthActor ;
                rdfs:range xsd:string ;
                rdfs:comment "The familly name of a health actor."@en ;
                rdfs:label "last name"@en .


###  https://saref.etsi.org/saref4ehaw/latency
s4ehaw:latency rdf:type owl:DatatypeProperty ;
               rdfs:domain s4ehaw:MeasurementFunction ;
               rdfs:range xsd:float ;
               rdfs:comment "The latency is the time interval between the stimulation and response of a measurement function (in ms)."@en ;
               rdfs:label "latency"@en .


###  https://saref.etsi.org/saref4ehaw/lifetime
s4ehaw:lifetime rdf:type owl:DatatypeProperty ;
                rdfs:domain s4ehaw:Ban ;
                rdfs:range xsd:float ;
                rdfs:comment "The BAN lifetime (in month), e.g. BAN for entertainment purposes should have a lifetime of weeks or few years whereas BAN dedicated for assisted living or anomaly monitoring should last for many years."@en ;
                rdfs:label "lifetime"@en .


###  https://saref.etsi.org/saref4ehaw/maximumFlash
s4ehaw:maximumFlash rdf:type owl:DatatypeProperty ;
                    rdfs:domain s4ehaw:ComputingPower ;
                    rdfs:range xsd:long ;
                    rdfs:comment "Indicates the maximum flash memory space (in byte) of a health device."@en ;
                    rdfs:label "maximum flash"@en .


###  https://saref.etsi.org/saref4ehaw/maximumRam
s4ehaw:maximumRam rdf:type owl:DatatypeProperty ;
                  rdfs:domain s4ehaw:ComputingPower ;
                  rdfs:range xsd:long ;
                  rdfs:comment "Indicates the maximum volatile memory space (in byte) of a health device."@en ;
                  rdfs:label "maximum ram"@en .


###  https://saref.etsi.org/saref4ehaw/maximumValue
s4ehaw:maximumValue rdf:type owl:DatatypeProperty ;
                    rdfs:domain s4ehaw:ValidityConstraint ;
                    rdfs:range xsd:decimal ;
                    rdfs:comment "The maximum allowable value of a measurement."@en ;
                    rdfs:label "maximum value"@en .


###  https://saref.etsi.org/saref4ehaw/minimumValue
s4ehaw:minimumValue rdf:type owl:DatatypeProperty ;
                    rdfs:domain s4ehaw:ValidityConstraint ;
                    rdfs:range xsd:decimal ;
                    rdfs:comment "The minimum allowable value  of a measurement."@en ;
                    rdfs:label "minimum value"@en .


###  https://saref.etsi.org/saref4ehaw/modeName
s4ehaw:modeName rdf:type owl:DatatypeProperty ;
                rdfs:domain s4ehaw:Mode ;
                rdfs:range xsd:string ;
                rdfs:comment "The mode name of a device, e.g. sleeping."@en ;
                rdfs:label "mode name"@en .


###  https://saref.etsi.org/saref4ehaw/phenomena
s4ehaw:phenomena rdf:type owl:DatatypeProperty ;
                 rdfs:domain s4ehaw:Ban ;
                 rdfs:range xsd:string ;
                 rdfs:comment "The BAN monitors a specific phenomenon (burned calories during exercises, glucose level...)."@en ;
                 rdfs:label "phenomena"@en .


###  https://saref.etsi.org/saref4ehaw/phone
s4ehaw:phone rdf:type owl:DatatypeProperty ;
             rdfs:domain s4ehaw:HealthActor ;
             rdfs:range xsd:string ;
             rdfs:comment "The phone number of a health actor, in international format."@en ;
             rdfs:label "phone"@en .


###  https://saref.etsi.org/saref4ehaw/portNumber
s4ehaw:portNumber rdf:type owl:DatatypeProperty ;
                  rdfs:domain s4ehaw:ServiceGrounding ;
                  rdfs:range xsd:positiveInteger ;
                  rdfs:comment "The port number used to offer the service."@en ;
                  rdfs:label "port number"@en .


###  https://saref.etsi.org/saref4ehaw/postalAddress
s4ehaw:postalAddress rdf:type owl:DatatypeProperty ;
                     rdfs:domain s4ehaw:PhysicalLocation ;
                     rdfs:range xsd:string ;
                     rdfs:comment "Defines the postal address."@en ;
                     rdfs:label "postal address"@en .


###  https://saref.etsi.org/saref4ehaw/powerSourceType
s4ehaw:powerSourceType rdf:type owl:DatatypeProperty ;
                       rdfs:domain s4ehaw:PowerSource ;
                       rdfs:range xsd:string ;
                       rdfs:comment "The type of power source of a health device. It can be solar, battery, electricity..."@en ;
                       rdfs:label "power source type"@en .


###  https://saref.etsi.org/saref4ehaw/rechargeable
s4ehaw:rechargeable rdf:type owl:DatatypeProperty ;
                    rdfs:domain s4ehaw:PowerSource ;
                    rdfs:range xsd:boolean ;
                    rdfs:comment "This boolean variable indicates if the power source is rechargeable or not, e.g. a rechargeable battery."@en ;
                    rdfs:label "rechargeable"@en .


###  https://saref.etsi.org/saref4ehaw/remainingBatteryLevel
s4ehaw:remainingBatteryLevel rdf:type owl:DatatypeProperty ;
                             rdfs:domain s4ehaw:HealthDevice ;
                             rdfs:range xsd:long ;
                             rdfs:comment "The level of remaining battery (if any : in percent) for a health device. It is a dynamic attribute."@en ;
                             rdfs:label "remaining battery level"@en .


###  https://saref.etsi.org/saref4ehaw/sampleTime
s4ehaw:sampleTime rdf:type owl:DatatypeProperty ;
                  rdfs:domain s4ehaw:MeasurementFunction ;
                  rdfs:range xsd:int ;
                  rdfs:comment "The sample time of a measurement function (a discrete integer)."@en ;
                  rdfs:label "sample time"@en .


###  https://saref.etsi.org/saref4ehaw/sendingFrequency
s4ehaw:sendingFrequency rdf:type owl:DatatypeProperty ;
                        rdfs:domain s4ehaw:PeriodicBanCommunicationType ;
                        rdfs:range xsd:float ;
                        rdfs:comment "Defines the sending frequency (in ms), at an health device level, in case of pariodic BAN communication type."@en ;
                        rdfs:label "sending frequency"@en .


###  https://saref.etsi.org/saref4ehaw/serialNb
s4ehaw:serialNb rdf:type owl:DatatypeProperty ;
                rdfs:domain s4ehaw:HealthDevice ;
                rdfs:range xsd:string ;
                rdfs:comment "The serial number of a health device."@en ;
                rdfs:label "serial number"@en .


###  https://saref.etsi.org/saref4ehaw/serviceDescription
s4ehaw:serviceDescription rdf:type owl:DatatypeProperty ;
                          rdfs:domain s4ehaw:ServiceProfile ;
                          rdfs:range xsd:string ;
                          rdfs:comment "The service description should describe the offered service like e.g. heart rate measurement."@en ;
                          rdfs:label "service description"@en .


###  https://saref.etsi.org/saref4ehaw/serviceName
s4ehaw:serviceName rdf:type owl:DatatypeProperty ;
                   rdfs:domain s4ehaw:ServiceProfile ;
                   rdfs:range xsd:string ;
                   rdfs:comment "The service name identify the offered service, e.g heart rate."@en ;
                   rdfs:label "service name"@en .


###  https://saref.etsi.org/saref4ehaw/transmissionRate
s4ehaw:transmissionRate rdf:type owl:DatatypeProperty ;
                        rdfs:domain s4ehaw:Interface ;
                        rdfs:range xsd:float ;
                        rdfs:comment "The transmission rate of the interface, i.e. the number of bits transmitted per second (usually expressed in kbps or Mbps)."@en ;
                        rdfs:label "transmission rate"@en .


###  https://saref.etsi.org/saref4ehaw/velocity
s4ehaw:velocity rdf:type owl:DatatypeProperty ;
                rdfs:domain s4ehaw:DeviceCharacteristic ;
                rdfs:range xsd:float ;
                rdfs:comment "The velocity of a moving device (in m/s)."@en ;
                rdfs:label "velocity"@en .


#################################################################
#    Classes
#################################################################

###  http://purl.org/vocommons/voaf#Vocabulary
voaf:Vocabulary rdf:type owl:Class .


###  http://www.w3.org/ns/ssn/systems/Precision
ssn-system:Precision rdf:type owl:Class .


###  http://xmlns.com/foaf/0.1/Agent
foaf:Agent rdf:type owl:Class .


###  https://saref.etsi.org/core/Command
saref:Command rdf:type owl:Class .


###  https://saref.etsi.org/core/Device
saref:Device rdf:type owl:Class .


###  https://saref.etsi.org/core/Function
saref:Function rdf:type owl:Class .


###  https://saref.etsi.org/core/Measurement
saref:Measurement rdf:type owl:Class .


###  https://saref.etsi.org/core/NotifyCommand
saref:NotifyCommand rdf:type owl:Class .


###  https://saref.etsi.org/core/Property
saref:Property rdf:type owl:Class .


###  https://saref.etsi.org/core/Service
saref:Service rdf:type owl:Class .


###  https://saref.etsi.org/core/Task
saref:Task rdf:type owl:Class .


###  https://saref.etsi.org/core/UnitOfMeasure
saref:UnitOfMeasure rdf:type owl:Class .


###  https://saref.etsi.org/saref4ehaw/Activity
s4ehaw:Activity rdf:type owl:Class ;
                rdfs:comment "The activity of a patient/user, i.e. daily and nocturnal activities."@en ;
                rdfs:label "Activity"@en .


###  https://saref.etsi.org/saref4ehaw/AgeCategory
s4ehaw:AgeCategory rdf:type owl:Class ;
                   rdfs:comment "The age group of a health actor, e.g. old or young."@en ;
                   rdfs:label "Age category"@en .


###  https://saref.etsi.org/saref4ehaw/AlarmCommand
s4ehaw:AlarmCommand rdf:type owl:Class ;
                    rdfs:subClassOf saref:Command ;
                    rdfs:comment "A command corresponding to alarm sending."@en ;
                    rdfs:label "Alarm command"@en .


###  https://saref.etsi.org/saref4ehaw/Ban
s4ehaw:Ban rdf:type owl:Class ;
           rdfs:comment "Body Area Network."@en ;
           rdfs:label "BAN"@en .


###  https://saref.etsi.org/saref4ehaw/BanApplicationDomain
s4ehaw:BanApplicationDomain rdf:type owl:Class ;
                            rdfs:comment "The BAN application domain, e.g. healthcare, telemedicine, assisted living, sport training, safety and emergency..."@en ;
                            rdfs:label "BAN application domain"@en .


###  https://saref.etsi.org/saref4ehaw/BanCommunicationType
s4ehaw:BanCommunicationType rdf:type owl:Class ;
                            rdfs:comment "The BAN communication function type, i.e. periodic, event driven or on request."@en ;
                            rdfs:label "BAN Communication type"@en .


###  https://saref.etsi.org/saref4ehaw/BanHub
s4ehaw:BanHub rdf:type owl:Class ;
              rdfs:subClassOf s4ehaw:HealthDevice ;
              rdfs:comment "Hub of the BAN, mainly playing the role of both a data concentrator and a network gateway."@en ;
              rdfs:label "BAN hub"@en .


###  https://saref.etsi.org/saref4ehaw/BodySurfaceLocation
s4ehaw:BodySurfaceLocation rdf:type owl:Class ;
                           rdfs:subClassOf s4ehaw:Location ;
                           rdfs:comment "Defines a health device location in terms of a body surface position (i.e. on body health device)."@en ;
                           rdfs:label "Body surface location"@en .


###  https://saref.etsi.org/saref4ehaw/Caregiver
s4ehaw:Caregiver rdf:type owl:Class ;
                 rdfs:subClassOf s4ehaw:HealthActor ;
                 rdfs:comment "For caregivers modelling."@en ;
                 rdfs:label "Caregiver"@en .


###  https://saref.etsi.org/saref4ehaw/ChronicDisease
s4ehaw:ChronicDisease rdf:type owl:Class ;
                      rdfs:comment "For chronic disease modelling, e.g. diabetes, asthma..."@en ;
                      rdfs:label "Chronic disease"@en .


###  https://saref.etsi.org/saref4ehaw/CommunicationProtocol
s4ehaw:CommunicationProtocol rdf:type owl:Class ;
                             rdfs:comment "The communication protocol, e.g. BLE, serial, Ethernet..."@en ;
                             rdfs:label "Communication protocol"@en .


###  https://saref.etsi.org/saref4ehaw/ComputingPower
s4ehaw:ComputingPower rdf:type owl:Class ;
                      rdfs:comment "The computing power capabilities of a Health device."@en ;
                      rdfs:label "Computing power"@en .


###  https://saref.etsi.org/saref4ehaw/Contact
s4ehaw:Contact rdf:type owl:Class ;
               owl:equivalentClass s4ehaw:HealthActor ;
               rdfs:comment "A BAN has one or multiple contacts, i.e. some health actors, e.g. the patient or user that is monitored through this BAN, the caregiver that is using this BAN for monitoring purposes..."@en ;
               rdfs:label "Contact"@en .


###  https://saref.etsi.org/saref4ehaw/DailyActivity
s4ehaw:DailyActivity rdf:type owl:Class ;
                     rdfs:subClassOf s4ehaw:Activity ;
                     rdfs:comment "The patient/user activities that occur during daytime."@en ;
                     rdfs:label "Daily activity"@en .


###  https://saref.etsi.org/saref4ehaw/Data
s4ehaw:Data rdf:type owl:Class ;
            rdfs:comment "A function has one or many data, for example a tracking function shall include latitude, longitude and speed data."@en ;
            rdfs:label "Data"@en .


###  https://saref.etsi.org/saref4ehaw/DataConstraint
s4ehaw:DataConstraint rdf:type owl:Class ;
                      rdfs:comment "The Data constraints, e.g. validity, legal..."@en ;
                      rdfs:label "Data constraint"@en .


###  https://saref.etsi.org/saref4ehaw/DeviceCharacteristic
s4ehaw:DeviceCharacteristic rdf:type owl:Class ;
                            rdfs:comment "A health device has device characteristic describing the physical characteristics of the health device."@en ;
                            rdfs:label "Device characteristic"@en .


###  https://saref.etsi.org/saref4ehaw/EventDrivenBanCommunicationType
s4ehaw:EventDrivenBanCommunicationType rdf:type owl:Class ;
                                       rdfs:subClassOf s4ehaw:BanCommunicationType ;
                                       rdfs:comment "BAN communication function way of working of the type event driven."@en ;
                                       rdfs:label "Event driven BAN communication type"@en .


###  https://saref.etsi.org/saref4ehaw/FunctionalDevice
s4ehaw:FunctionalDevice rdf:type owl:Class ;
                        rdfs:subClassOf saref:Device ;
                        rdfs:comment "Functional Devices are non-purely eHealth/ageing-well devices that can be used for modelling/detecting activities or behaviours of patients/users, like for example beacons that can detect indoor positioning of a patient in a house."@en ;
                        rdfs:label "Functional device"@en .


###  https://saref.etsi.org/saref4ehaw/Habit
s4ehaw:Habit rdf:type owl:Class ;
             rdfs:comment "Defined for users (that can in particular be patients) habits modelling, e.g. smoking, alcohol drinking, overeating, undereating..."@en ;
             rdfs:label "Habit"@en .


###  https://saref.etsi.org/saref4ehaw/HealthActor
s4ehaw:HealthActor rdf:type owl:Class ;
                   rdfs:subClassOf foaf:Agent ;
                   rdfs:comment "The eHealth actors like e.g. caregivers, patients, users, helpers..."@en ;
                   rdfs:label "Health actor"@en .


###  https://saref.etsi.org/saref4ehaw/HealthActuator
s4ehaw:HealthActuator rdf:type owl:Class ;
                      rdfs:subClassOf s4ehaw:HealthDevice ;
                      rdfs:comment "Health-related Actuator, equivalent to SAREF Actuator."@en ;
                      rdfs:label "Health actuator"@en .


###  https://saref.etsi.org/saref4ehaw/HealthDevice
s4ehaw:HealthDevice rdf:type owl:Class ;
                    rdfs:subClassOf saref:Device ;
                    rdfs:comment "Health devices, e.g. BAN hub, health sensor/actuator/Wereable."@en ;
                    rdfs:label "Health Device"@en .


###  https://saref.etsi.org/saref4ehaw/HealthSensor
s4ehaw:HealthSensor rdf:type owl:Class ;
                    rdfs:subClassOf s4ehaw:HealthDevice ;
                    rdfs:comment "Health-related Sensor, equivalent to SAREF Sensor."@en ;
                    rdfs:label "Health sensor"@en .


###  https://saref.etsi.org/saref4ehaw/HealthWearable
s4ehaw:HealthWearable rdf:type owl:Class ;
                      rdfs:subClassOf s4ehaw:HealthDevice ;
                      rdfs:comment "Health-related Wearable, equivalent to SAREF4WEAR Wearable."@en ;
                      rdfs:label "Health wereable"@en .


###  https://saref.etsi.org/saref4ehaw/Helper
s4ehaw:Helper rdf:type owl:Class ;
              rdfs:subClassOf s4ehaw:HealthActor ;
              rdfs:comment "Helper of patients/users, e.g. a patient's relative."@en ;
              rdfs:label "Helper"@en .


###  https://saref.etsi.org/saref4ehaw/Impairment
s4ehaw:Impairment rdf:type owl:Class ;
                  rdfs:comment "Defined for users (that can in particular be patients) impairments modelling, e.g. aural impairment, skeletal impairment, ocular impairment, mobility impairment, intellectual impairment. Those non exhaustive impairments are compatible with the World Health Organization classification."@en ;
                  rdfs:label "Impairment"@en .


###  https://saref.etsi.org/saref4ehaw/ImplantLocation
s4ehaw:ImplantLocation rdf:type owl:Class ;
                       rdfs:subClassOf s4ehaw:Location ;
                       rdfs:comment "Implant Device (i.e. in body health device) position."@en ;
                       rdfs:label "Implant location"@en .


###  https://saref.etsi.org/saref4ehaw/Interface
s4ehaw:Interface rdf:type owl:Class ;
                 rdfs:comment "Used for modelling the interfaces of a health device (e.g. Bluetooth, UWB, IEEE 802.15.6, serial interface...)."@en ;
                 rdfs:label "Interface"@en .


###  https://saref.etsi.org/saref4ehaw/LegalConstraint
s4ehaw:LegalConstraint rdf:type owl:Class ;
                       rdfs:subClassOf s4ehaw:DataConstraint ;
                       rdfs:comment "An empty container for describing the legal constraints a data can be submitted to, like e.g. anonymization."@en ;
                       rdfs:label "Legal constraint"@en .


###  https://saref.etsi.org/saref4ehaw/Location
s4ehaw:Location rdf:type owl:Class ;
                rdfs:comment "The location, i.e. a position against the body (on - body surface – or in the body – implant –) and a physical location (i.e. a postal address and/or a current geolocation when available)."@en ;
                rdfs:label "Location"@en .


###  https://saref.etsi.org/saref4ehaw/MeasurementCollectionSession
s4ehaw:MeasurementCollectionSession rdf:type owl:Class ;
                                    rdfs:subClassOf saref:Task ;
                                    rdfs:comment "Task in which a health actor (mainly a patient or a user) is subject of measurement collection (recording) by both some measurement-related health Device (e.g. Sensor, Wearable, ECG Device...) and a health actor (mainly a caregiver)."@en ;
                                    rdfs:label "Measurement collection session"@en .


###  https://saref.etsi.org/saref4ehaw/MeasurementFunction
s4ehaw:MeasurementFunction rdf:type owl:Class ;
                           rdfs:subClassOf saref:Function ;
                           rdfs:comment "The functionality necessary to accomplish the measurement task for which a measurement-related health Device (e.g. Sensor, Wearable, ECG Device...) is designed for, e.g. a heart rate measurement function."@en ;
                           rdfs:label "Measurement function"@en .


###  https://saref.etsi.org/saref4ehaw/Mode
s4ehaw:Mode rdf:type owl:Class ;
            rdfs:comment "The dynamic characteristics of a eHealth Device that vary during its lifetime or its BAN lifetime."@en ;
            rdfs:label "Mode"@en .


###  https://saref.etsi.org/saref4ehaw/NocturnalActivity
s4ehaw:NocturnalActivity rdf:type owl:Class ;
                         rdfs:subClassOf s4ehaw:Activity ;
                         rdfs:comment "The patient/user activities that occur during the night."@en ;
                         rdfs:label "Nocturnal activity"@en .


###  https://saref.etsi.org/saref4ehaw/OnRequestBanCommunicationType
s4ehaw:OnRequestBanCommunicationType rdf:type owl:Class ;
                                     rdfs:subClassOf s4ehaw:BanCommunicationType ;
                                     rdfs:comment "BAN communication function way of working of the type on request."@en ;
                                     rdfs:label "On request BAN communication type"@en .


###  https://saref.etsi.org/saref4ehaw/OperatingConstraint
s4ehaw:OperatingConstraint rdf:type owl:Class ;
                           rdfs:comment "An empty container for describing the operating constraints of a device, e.g. recommended humidity and temperature range..."@en ;
                           rdfs:label "Operating constraint"@en .


###  https://saref.etsi.org/saref4ehaw/Patient
s4ehaw:Patient rdf:type owl:Class ;
               rdfs:subClassOf s4ehaw:User ;
               rdfs:comment "A user of the type patient, i.e. a cared-for person by one or multiple caregivers."@en ;
               rdfs:label "Patient"@en .


###  https://saref.etsi.org/saref4ehaw/PeriodicBanCommunicationType
s4ehaw:PeriodicBanCommunicationType rdf:type owl:Class ;
                                    rdfs:subClassOf s4ehaw:BanCommunicationType ;
                                    rdfs:comment "BAN communication function way of working of the type periodic."@en ;
                                    rdfs:label "Periodic BAN communication type"@en .


###  https://saref.etsi.org/saref4ehaw/PhysicalLocation
s4ehaw:PhysicalLocation rdf:type owl:Class ;
                        rdfs:subClassOf s4ehaw:Location ;
                        rdfs:comment "The physical location, i.e. a postal address and a geolocation when available."@en ;
                        rdfs:label "Physical location"@en .


###  https://saref.etsi.org/saref4ehaw/Posture
s4ehaw:Posture rdf:type owl:Class ;
               rdfs:subClassOf saref:Property ;
               rdfs:comment "The posture of a health actor (mainly a patient or a user), e.g. exercising, lying, running, sitting, walking..."@en ;
               rdfs:label "Posture"@en .


###  https://saref.etsi.org/saref4ehaw/PowerSource
s4ehaw:PowerSource rdf:type owl:Class ;
                   rdfs:comment "The power sources of a health device, mainly describing energy source and battery related capabilities of the health device (number of power source, source type, rechargeable or not...)."@en ;
                   rdfs:label "Power source"@en .


###  https://saref.etsi.org/saref4ehaw/ReminderCommand
s4ehaw:ReminderCommand rdf:type owl:Class ;
                       rdfs:subClassOf saref:NotifyCommand ;
                       rdfs:comment "Command used for sending reminder notifications to health actors, e.g. patients, users or Caregivers."@en ;
                       rdfs:label "Reminder command"@en .


###  https://saref.etsi.org/saref4ehaw/ResponsibleParty
s4ehaw:ResponsibleParty rdf:type owl:Class ;
                        rdfs:subClassOf s4ehaw:HealthActor ;
                        rdfs:comment "The legal entity responsible for a BAN, i.e. to contact in case of problem."@en ;
                        rdfs:label "Responsible party"@en .


###  https://saref.etsi.org/saref4ehaw/ServiceGrounding
s4ehaw:ServiceGrounding rdf:type owl:Class ;
                        rdfs:comment "How to access the service."@en ;
                        rdfs:label "Service grounding"@en .


###  https://saref.etsi.org/saref4ehaw/ServiceProcess
s4ehaw:ServiceProcess rdf:type owl:Class ;
                      rdfs:comment "How the service works."@en ;
                      rdfs:label "Service process"@en .


###  https://saref.etsi.org/saref4ehaw/ServiceProfile
s4ehaw:ServiceProfile rdf:type owl:Class ;
                      rdfs:comment "What the service does."@en ;
                      rdfs:label "Service profile"@en .


###  https://saref.etsi.org/saref4ehaw/TimeSeriesMeasurement
s4ehaw:TimeSeriesMeasurement rdf:type owl:Class ;
                             rdfs:subClassOf saref:Measurement ,
                                             [ rdf:type owl:Restriction ;
                                               owl:onProperty s4envi:hasFrequencyMeasurement ;
                                               owl:allValuesFrom s4envi:FrequencyMeasurement
                                             ] ,
                                             [ rdf:type owl:Restriction ;
                                               owl:onProperty s4ehaw:hasValues ;
                                               owl:allValuesFrom xsd:decimal
                                             ] ;
                             rdfs:comment "A sequence of data in a successive equally spaced points in time. The O&M ontology (ISO 19156) defines Time Series Observation  as an “observation whose result is a time-series”, while both Hl7 aECG and DICOM standards define the Series element as a sequence of data sharing a common frame of reference. In SAREF4health this concept is termed as Time Series Measurements since this sequence of data refers to time series measured by a health device."@en ;
                             rdfs:label "Time series measurement"@en .


###  https://saref.etsi.org/saref4ehaw/User
s4ehaw:User rdf:type owl:Class ;
            rdfs:subClassOf s4ehaw:HealthActor ;
            rdfs:comment "A health actor (patient included) that can be equiped with BANs or health devices for monitoring, control, care (specific case of patients) or support purposes."@en ;
            rdfs:label "User"@en .


###  https://saref.etsi.org/saref4ehaw/ValidityConstraint
s4ehaw:ValidityConstraint rdf:type owl:Class ;
                          rdfs:subClassOf s4ehaw:DataConstraint ;
                          rdfs:comment "Data may have validity constraint such as allowable value range."@en ;
                          rdfs:label "Validity constraint"@en .


###  https://saref.etsi.org/saref4envi/Frequency
s4envi:Frequency rdf:type owl:Class .


###  https://saref.etsi.org/saref4envi/FrequencyMeasurement
s4envi:FrequencyMeasurement rdf:type owl:Class ;
                            rdfs:comment "Represents the measured value made over a frequency property. It is also linked to the frequency unit of measure in which the value is expressed and the timestamp of the measurement."@en ;
                            rdfs:isDefinedBy s4envi: ;
                            rdfs:label "Frequency measurement"@en .


###  https://saref.etsi.org/saref4envi/FrequencyUnit
s4envi:FrequencyUnit rdf:type owl:Class .


#################################################################
#    Individuals
#################################################################

###  https://saref.etsi.org/saref4ehaw/AlcoholDrinking
s4ehaw:AlcoholDrinking rdf:type owl:NamedIndividual ,
                                s4ehaw:Habit ;
                       rdfs:comment "Alcohol drinking habit (User level)."@en ;
                       rdfs:label "Alcohol drinking"@en .


###  https://saref.etsi.org/saref4ehaw/ArmpitLocation
s4ehaw:ArmpitLocation rdf:type owl:NamedIndividual ,
                               s4ehaw:BodySurfaceLocation ;
                      rdfs:comment "Armpit location, a user body surface location."@en ;
                      rdfs:label "Armpit location"@en .


###  https://saref.etsi.org/saref4ehaw/AssistedLiving
s4ehaw:AssistedLiving rdf:type owl:NamedIndividual ,
                               s4ehaw:BanApplicationDomain ;
                      rdfs:comment "Assisted living sub-domain for BAN application."@en ;
                      rdfs:label "Assisted living"@en .


###  https://saref.etsi.org/saref4ehaw/Asthma
s4ehaw:Asthma rdf:type owl:NamedIndividual ,
                       s4ehaw:ChronicDisease ;
              rdfs:comment "Asthma, a chronical disease that some users can have."@en ;
              rdfs:label "Asthma"@en .


###  https://saref.etsi.org/saref4ehaw/AuralImpairment
s4ehaw:AuralImpairment rdf:type owl:NamedIndividual ,
                                s4ehaw:Impairment ;
                       rdfs:comment "Aural impairment (User level), i.e. impairments of auditory sensitivity."@en ;
                       rdfs:label "Aural impairment"@en .


###  https://saref.etsi.org/saref4ehaw/Diabetes
s4ehaw:Diabetes rdf:type owl:NamedIndividual ,
                         s4ehaw:ChronicDisease ;
                rdfs:comment "Diabetes, a chronical disease that some users can have."@en ;
                rdfs:label "Diabetes"@en .


###  https://saref.etsi.org/saref4ehaw/Emergency
s4ehaw:Emergency rdf:type owl:NamedIndividual ,
                          s4ehaw:BanApplicationDomain ;
                 rdfs:comment "Emergency sub-domain for BAN application."@en ;
                 rdfs:label "Emergency"@en .


###  https://saref.etsi.org/saref4ehaw/Exercising
s4ehaw:Exercising rdf:type owl:NamedIndividual ,
                           s4ehaw:Posture ;
                  rdfs:comment "Posture of user doing exercises."@en ;
                  rdfs:label "Exercising"@en .


###  https://saref.etsi.org/saref4ehaw/Healthcare
s4ehaw:Healthcare rdf:type owl:NamedIndividual ,
                           s4ehaw:BanApplicationDomain ;
                  rdfs:comment "Healthcare domain for BAN application."@en ;
                  rdfs:label "Healthcare"@en .


###  https://saref.etsi.org/saref4ehaw/IntellectualImpairment
s4ehaw:IntellectualImpairment rdf:type owl:NamedIndividual ,
                                       s4ehaw:Impairment ;
                              rdfs:comment "Skeletal impairment (User level), e.g. ..."@en ;
                              rdfs:label "Intellectual impairment"@en .


###  https://saref.etsi.org/saref4ehaw/Lying
s4ehaw:Lying rdf:type owl:NamedIndividual ,
                      s4ehaw:Posture ;
             rdfs:comment "Posture of a lying user."@en ;
             rdfs:label "Lying"@en .


###  https://saref.etsi.org/saref4ehaw/MobilityImpairment
s4ehaw:MobilityImpairment rdf:type owl:NamedIndividual ,
                                   s4ehaw:Impairment ;
                          rdfs:comment "Mobility impairment (User level)."@en ;
                          rdfs:label "Mobility impairment"@en .


###  https://saref.etsi.org/saref4ehaw/OcularImpairment
s4ehaw:OcularImpairment rdf:type owl:NamedIndividual ,
                                 s4ehaw:Impairment ;
                        rdfs:comment "Ocular impairment (User level), i.e. impamnents of visual acuity."@en ,
                                     "Ocular impairment (User level)."@en ;
                        rdfs:label "Ocular impairment"@en .


###  https://saref.etsi.org/saref4ehaw/Old
s4ehaw:Old rdf:type owl:NamedIndividual ,
                    s4ehaw:AgeCategory ;
           rdfs:comment "Old, one user age category."@en ;
           rdfs:label "Old"@en .


###  https://saref.etsi.org/saref4ehaw/Overeating
s4ehaw:Overeating rdf:type owl:NamedIndividual ,
                           s4ehaw:Habit ;
                  rdfs:comment "Overeating habit (User level)."@en ;
                  rdfs:label "Overeating"@en .


###  https://saref.etsi.org/saref4ehaw/PervasiveComputing
s4ehaw:PervasiveComputing rdf:type owl:NamedIndividual ,
                                   s4ehaw:BanApplicationDomain ;
                          rdfs:comment "Pervasive computing sub-domain for BAN application."@en ;
                          rdfs:label "Pervasive computing"@en .


###  https://saref.etsi.org/saref4ehaw/Prevention
s4ehaw:Prevention rdf:type owl:NamedIndividual ,
                           s4ehaw:BanApplicationDomain ;
                  rdfs:comment "Prevention sub-domain (e.g. preventive health) for BAN application."@en ;
                  rdfs:label "Prevention"@en .


###  https://saref.etsi.org/saref4ehaw/Running
s4ehaw:Running rdf:type owl:NamedIndividual ,
                        s4ehaw:Posture ;
               rdfs:comment "Posture of a running user."@en ;
               rdfs:label "Running"@en .


###  https://saref.etsi.org/saref4ehaw/Safety
s4ehaw:Safety rdf:type owl:NamedIndividual ,
                       s4ehaw:BanApplicationDomain ;
              rdfs:comment "Safety sub-domain for BAN application."@en ;
              rdfs:label "Safety"@en .


###  https://saref.etsi.org/saref4ehaw/Sitting
s4ehaw:Sitting rdf:type owl:NamedIndividual ,
                        s4ehaw:Posture ;
               rdfs:comment "Posture of a sitting user."@en ;
               rdfs:label "Sitting"@en .


###  https://saref.etsi.org/saref4ehaw/SkeletalImpairment
s4ehaw:SkeletalImpairment rdf:type owl:NamedIndividual ,
                                   s4ehaw:Impairment ;
                          rdfs:comment "Skeletal impairment (User level), e.g. of head and trunk regions, limbs..."@en ;
                          rdfs:label "Skeletal impairment"@en .


###  https://saref.etsi.org/saref4ehaw/Smoking
s4ehaw:Smoking rdf:type owl:NamedIndividual ,
                        s4ehaw:Habit ;
               rdfs:comment "Smoking habit (User level)."@en ;
               rdfs:label "Smoking"@en .


###  https://saref.etsi.org/saref4ehaw/SportTraining
s4ehaw:SportTraining rdf:type owl:NamedIndividual ,
                              s4ehaw:BanApplicationDomain ;
                     rdfs:comment "Sport training sub-domain for BAN application."@en ;
                     rdfs:label "Sport Training"@en .


###  https://saref.etsi.org/saref4ehaw/Telemedicine
s4ehaw:Telemedicine rdf:type owl:NamedIndividual ,
                             s4ehaw:BanApplicationDomain ;
                    rdfs:comment "Telemedicine sub-domain for BAN application."@en ;
                    rdfs:label "Telemedicine"@en .


###  https://saref.etsi.org/saref4ehaw/Undereating
s4ehaw:Undereating rdf:type owl:NamedIndividual ,
                            s4ehaw:Habit ;
                   rdfs:comment "Undereating habit (User level)."@en ;
                   rdfs:label "Undereating"@en .


###  https://saref.etsi.org/saref4ehaw/Walking
s4ehaw:Walking rdf:type owl:NamedIndividual ,
                        s4ehaw:Posture ;
               rdfs:comment "Posture of a walking user."@en ;
               rdfs:label "Walking"@en .


###  https://saref.etsi.org/saref4ehaw/WristLocation
s4ehaw:WristLocation rdf:type owl:NamedIndividual ,
                              s4ehaw:BodySurfaceLocation ;
                     rdfs:comment "Wrist, a user body surface location."@en ;
                     rdfs:label "Wrist location"@en .


###  https://saref.etsi.org/saref4ehaw/Young
s4ehaw:Young rdf:type owl:NamedIndividual ,
                      s4ehaw:AgeCategory ;
             rdfs:comment "Young, one user age category."@en ;
             rdfs:label "Young"@en .


###  Generated by the OWL API (version 4.5.29.2024-05-13T12:11:03Z) https://github.com/owlcs/owlapi
